Repeat all proof

examples/repeat/Add1.v
@@ -6,7 +6,7 @@ Require Import Behavior.
 Require Import ModSem.
 Require Import Skeleton.
 Require Import PCM.
-Require Import HoareDef.
+Require Import HoareDef OpenDef.
 Require Import ProofMode.
 Require Import STB.
 
@@ -41,25 +41,25 @@ Section PROOF.
         Ret (Vint (n + m)%Z)
     .
 
-    Definition AddSbtb: list (gname * fspecbody) :=
-      [("succ", mk_specbody succ_spec (fun _ => trigger (Choose _)));
-      ("add", mk_specbody fspec_trivial (cfunU add_body))].
+    Definition AddSbtb: list (gname * kspecbody) :=
+      [("succ", mk_kspecbody succ_spec (fun _ => triggerUB) (fun _ => triggerNB));
+      ("add", ksb_trivial (cfunU add_body))].
 
-    Definition SAddSem: SModSem.t := {|
-      SModSem.fnsems := AddSbtb;
-      SModSem.mn := "Add";
-      SModSem.initial_mr := ε;
-      SModSem.initial_st := tt↑;
+    Definition KAddSem: KModSem.t := {|
+      KModSem.fnsems := AddSbtb;
+      KModSem.mn := "Add";
+      KModSem.initial_mr := ε;
+      KModSem.initial_st := tt↑;
     |}
     .
   End SKENV.
 
-  Definition SAdd: SMod.t := {|
-    SMod.get_modsem := fun _ => SAddSem;
-    SMod.sk := [("succ", Sk.Gfun); ("add", Sk.Gfun)];
+  Definition KAdd: KMod.t := {|
+    KMod.get_modsem := fun _ => KAddSem;
+    KMod.sk := [("succ", Sk.Gfun); ("add", Sk.Gfun)];
   |}
   .
 
-  Definition Add: Mod.t := (SMod.to_tgt GlobalStb) SAdd.
+  Definition Add: Mod.t := (KMod.transl_tgt GlobalStb) KAdd.
 
 End PROOF.
