examples/repeat/Repeat1.v
@@ -6,7 +6,7 @@ Require Import Behavior.
 Require Import ModSem.
 Require Import Skeleton.
 Require Import PCM.
-Require Import HoareDef.
+Require Import HoareDef OpenDef.
 Require Import ProofMode.
 Require Import STB.
 
@@ -50,23 +50,24 @@ Section PROOF.
                      )
                 )).
 
-    Definition RepeatSbtb: list (gname * fspecbody) :=[("repeat", mk_specbody repeat_spec (fun _ => trigger (Choose _)))].
+    Definition RepeatSbtb: list (gname * kspecbody) :=
+      [("repeat", mk_kspecbody repeat_spec (fun _ => triggerUB) (fun _ => triggerNB))].
 
-    Definition SRepeatSem: SModSem.t := {|
-      SModSem.fnsems := RepeatSbtb;
-      SModSem.mn := "Repeat";
-      SModSem.initial_mr := ε;
-      SModSem.initial_st := tt↑;
+    Definition KRepeatSem: KModSem.t := {|
+      KModSem.fnsems := RepeatSbtb;
+      KModSem.mn := "Repeat";
+      KModSem.initial_mr := ε;
+      KModSem.initial_st := tt↑;
     |}
     .
   End SKENV.
 
-  Definition SRepeat: SMod.t := {|
-    SMod.get_modsem := SRepeatSem;
-    SMod.sk := [("repeat", Sk.Gfun)];
+  Definition KRepeat: KMod.t := {|
+    KMod.get_modsem := KRepeatSem;
+    KMod.sk := [("repeat", Sk.Gfun)];
   |}
   .
 
-  Definition Repeat: Mod.t := (SMod.to_tgt GlobalStb) SRepeat.
+  Definition Repeat: Mod.t := (KMod.transl_tgt GlobalStb) KRepeat.
 
 End PROOF.
