examples/repeat/RepeatAll.v
@@ -1,4 +1,5 @@
-Require Import HoareDef STB Add1 Repeat1 SimModSem.
+Require Import HoareDef OpenDef Open STB.
+Require Import Add0 Repeat0 Add1 Repeat1 Add01proof Repeat01proof.
 Require Import Coqlib.
 Require Import ImpPrelude.
 Require Import Skeleton.
@@ -26,18 +27,19 @@ Set Implicit Arguments.
 
 Local Open Scope nat_scope.
 
-Section EQUATION.
-  Context `{Σ: GRA.t}.
+Section PROOF.
+  Let Σ: GRA.t := GRA.of_list [].
+  Local Existing Instance Σ.
 
   Let FunStb: Sk.t -> gname -> option fspec :=
     fun sk => to_stb [("succ", succ_spec)].
 
   Let GlobalStb: Sk.t -> gname -> option fspec :=
-    fun sk => to_stb (SMod.get_stb [Add1.SAdd; Repeat1.SRepeat FunStb] sk).
+    fun sk => to_closed_stb (KMod.get_stb [Add1.KAdd; Repeat1.KRepeat FunStb] sk).
 
   Let FunStb_incl: forall sk,
       stb_incl (FunStb sk) (GlobalStb sk).
-  Proof. stb_incl_tac. Qed.
+  Proof. i. etrans; [|eapply to_closed_stb_weaker]. stb_incl_tac. Qed.
 
   Let GlobalStb_repeat: forall sk,
       fn_has_spec (GlobalStb sk) "repeat" (Repeat1.repeat_spec FunStb sk).
@@ -46,4 +48,16 @@ Section EQUATION.
   Let FunStb_succ: forall sk,
       fn_has_spec (FunStb sk) "succ" (Add1.succ_spec).
   Proof. ii. econs; ss. refl. Qed.
-End EQUATION.
+
+  Let prog_tgt := [Add0.Add; Repeat0.Repeat].
+  Let prog_src := KMod.transl_src_list [Add1.KAdd; Repeat1.KRepeat FunStb].
+
+  Theorem correct: refines2 prog_tgt prog_src.
+  Proof.
+    etrans; cycle 1.
+    { eapply adequacy_open. i. exists ε. splits; ss. g_wf_tac. }
+    eapply refines2_cons.
+    { eapply Add01proof.correct; et. }
+    { eapply Repeat01proof.correct; et. }
+  Qed.
+End PROOF.
